% https://topanswers.xyz/tex?q=1325#a1564
\documentclass[xcolor={rgb}]{beamer}
\beamertemplatenavigationsymbolsempty
\setbeamersize{text margin left=10mm,text margin right=5mm} 
\setbeamertemplate{frametitle}[default][center]
\newcommand{\var}[1]{\operatorname{var}{\!#1}}
\begin{document}
\begin{frame}[t]
{\small\begin{align*}
\var(X) &= 0 + \var{\left(g(a) \sum_{j\in[n]\backslash\{a\}} f_j\cdot g(j) Y_j\right)}\\ 
&= \mathbb{E}\left( g(a)^2 \sum_{j\in[n]\backslash\{a\}} f^2_j Y^2_j + g(a)^2 \sum_{j\in[n]\backslash\{a\}} \right) - \left(\sum_{j\in[n]\backslash\{a\}} f_j \mathbb{E}[g(a)g(j)Y_j]\right)
\end{align*}}
\end{frame}

\begin{frame}[t]
\begin{align*}
\var(X) = & 0 + \var{\left(g(a) \sum_{j\in[n]\backslash\{a\}} f_j\cdot g(j) Y_j\right)}\\ 
= & \mathbb{E}\left( g(a)^2 \sum_{j\in[n]\backslash\{a\}} f^2_j Y^2_j + g(a)^2 \sum_{j\in[n]\backslash\{a\}} \right) -\\
&- \left(\sum_{j\in[n]\backslash\{a\}} f_j \mathbb{E}[g(a)g(j)Y_j]\right)
\end{align*}
\end{frame}
\end{document}